veric/semax_call.v
@@ -28,44 +28,6 @@ Section mpred.
 
 Context `{!VSTGS OK_ty Σ} {OK_spec : ext_spec OK_ty} {CS: compspecs}.
 
-Lemma tc_environ_make_args':
- forall argsig retsig bl rho Delta
-   (Htc : tc_environ Delta rho),
-  tc_exprlist Delta (snd (split argsig)) bl rho
-  ⊢ ⌜tc_environ (funsig_tycontext (argsig, retsig)) (make_args (map fst argsig)
-         (eval_exprlist (snd (split argsig)) bl rho) rho)⌝.
-Proof.
-  intros.
-  rewrite /tc_environ /tc_exprlist /=.
-  revert bl; induction argsig; destruct bl as [ | b bl]; simpl; intros; unfold_lift.
-  * iPureIntro; intros _; split3; hnf; try split; intros; try rewrite /funsig_tycontext ?Maps.PTree.gempty // in H |- *.
-    destruct H as [? H]; inv H.
-  * iPureIntro; done.
-  * destruct a as [i ti]; simpl.
-    destruct (split argsig) eqn:?; simpl.
-    unfold_lift; iPureIntro; inversion 1.
-  * destruct a as [i ti]; simpl.
-    destruct (split argsig) eqn:?; simpl.
-    specialize (IHargsig bl).
-    rewrite /typecheck_expr; fold typecheck_expr.
-    rewrite !denote_tc_assert_andp.
-    unfold_lift.
-    rewrite IHargsig; clear IHargsig.
-    iIntros "(H & (%Ht & % & %))".
-    unfold typecheck_environ; simpl.
-    rewrite tc_val_sem_cast //.
-    iDestruct "H" as %?%tc_val_tc_val'; iPureIntro.
-    split3; auto.
-    unfold typecheck_temp_environ; intros ?? Hset.
-    destruct (ident_eq i id).
-    - subst.
-      rewrite Maps.PTree.gss in Hset; inv Hset.
-      rewrite lookup_insert; eauto.
-    - rewrite lookup_insert_ne //.
-      apply (Ht id ty).
-      rewrite Maps.PTree.gso // in Hset.
-Qed.
-
 (* Scall *)
 
 Definition substopt {A} (ret: option ident) (v: environ -> val) (P: environ -> A)  : environ -> A :=
@@ -168,6 +130,65 @@ exists x. split. auto.
 eapply smaller_temps_exists'; eauto.
 Qed.
 
+(*Lemma semax_call_typecheck_environ:
+  forall (Delta : tycontext) (args: list val) (psi : genv)
+           m (b : block) (f : function)
+     (H17 : list_norepet (map fst (fn_params f) ++ map fst (fn_temps f)))
+     (H17' : list_norepet (map fst (fn_vars f)))
+     (H16 : Genv.find_funct_ptr psi b = Some (Internal f))
+     (ve' : env) m' (te' : temp_env)
+     (H15 : alloc_variables psi empty_env m (fn_vars f) ve' m')
+     (TC5: typecheck_glob_environ psi (glob_types Delta))
+     (TC8 : tc_vals (snd (split (fn_params f))) args)
+     (H21 : bind_parameter_temps (fn_params f) args
+              (create_undef_temps (fn_temps f)) = Some te'),
+   typecheck_environ (func_tycontext' f Delta)
+      (ge_of psi, ve', te').
+Proof.
+  intros.
+  pose (rho3 := mkEnviron (filter_genv psi) (make_venv ve') (make_tenv te')).
+  split3; auto.
+  - unfold typecheck_temp_environ; simpl; intros ?? H.
+    apply func_tycontext_t_sound in H; auto.
+    clear - H21 H TC8 H17.
+    destruct (in_dec (EqDec_prod _ _ _ _) (id, ty) (fn_params f)).
+    + forget (create_undef_temps (fn_temps f)) as temps.
+      rewrite snd_split in TC8.
+      generalize dependent temps. generalize dependent args. generalize dependent te'.
+      induction (fn_params f); intros; first done.
+      destruct a; simpl in *.
+      destruct args; first done.
+      destruct TC8 as [TC8' TC8].
+      clear H; destruct i as [H | H].
+      * inv H.
+        rewrite -> (pass_params_ni _ _ id _ _ H21)
+           by (inv H17; contradict H1; apply in_app; auto).
+        rewrite Maps.PTree.gss.
+        apply tc_val_tc_val' in TC8'; eauto.
+      * inv H17; eauto.
+    + destruct H as [? | H]; first done.
+      apply list_norepet_app in H17 as (? & ? & Hdisj).
+      rewrite -> (pass_params_ni _ _ id _ _ H21).
+      2: { intros; contradiction (Hdisj id id); auto.
+          rewrite in_map_iff; exists (id, ty); auto. }
+      clear - H; forget (fn_temps f) as temps; induction temps; first done.
+      destruct a; simpl in *.
+      destruct (eq_dec i id).
+      * subst; rewrite Maps.PTree.gss; eauto.
+        eexists; split; eauto; apply tc_val'_Vundef.
+      * rewrite Maps.PTree.gso //.
+        destruct H; [by inv H | eauto].
+  - rewrite /typecheck_var_environ /=; intros.
+    rewrite (func_tycontext_v_sound (fn_vars f) id ty); auto.
+    rewrite /Map.get /make_venv.
+    split.
+    + intros; eapply alloc_vars_lemma; eauto.
+      intros; apply Maps.PTree.gempty.
+    + intros (? & H); apply alloc_vars_match_venv in H15.
+      rewrite /match_venv /make_venv in H15.
+      specialize (H15 id); rewrite H // in H15.
+Qed.*)
+
 Definition tc_fn_return (Delta: tycontext) (ret: option ident) (t: type) :=
  match ret with
  | None => True%type
@@ -188,8 +209,9 @@ Lemma believe_exists_fundef:
   forall {CS}
     {b : block} {id_fun : ident} {psi : genv} {Delta : tycontext}
     {fspec: funspec}
+  (Findb : Genv.find_symbol (genv_genv psi) id_fun = Some b)
   (H3: (glob_specs Delta) !! id_fun = Some fspec),
-  believe(CS := CS) OK_spec Delta psi ∗ ⎡gvar id_fun b⎤ ⊢
+  believe(CS := CS) OK_spec Delta psi Delta ⊢
   ⌜∃ f : Clight.fundef,
    Genv.find_funct_ptr (genv_genv psi) b = Some f /\
    type_of_fundef f = type_of_funspec fspec⌝.
@@ -197,29 +219,20 @@ Proof.
   intros.
   destruct fspec as [[params retty] cc A E P Q].
   simpl.
-  iIntros "(Believe & g)".
-  iSpecialize ("Believe" with "[g]").
-  { iIntros "!>"; iExists id_fun; iFrame; eauto. }
+  iIntros "Believe".
+  iSpecialize ("Believe" with "[%]").
+  { exists id_fun; eauto. }
   iDestruct "Believe" as "[BE|BI]".
-  - iStopProof. rewrite -embed_pure; apply embed_mono.
-    rewrite /believe_external /=.
+  - rewrite /believe_external /=.
     if_tac; last done.
-    iIntros "BE".
-    destruct (Genv.find_funct_ptr psi b) eqn: Hf; last done.
+    destruct (Genv.find_funct_ptr psi b) eqn: Hf; last by rewrite embed_pure.
     iExists _; iSplit; first done.
-    destruct f as [ | ef sigargs sigret c'']; first done.
+    destruct f as [ | ef sigargs sigret c'']; first by rewrite embed_pure.
     iDestruct "BE" as ((Es & -> & ASD & _)) "(#? & _)"; inv Es; done.
   - iDestruct "BI" as (b' fu (? & WOB & ? & ? & ? & ? & [=] & ?)) "_"; iPureIntro.
     assert (b' = b) by congruence. subst b'.
     eexists; split; first done; simpl.
     unfold type_of_function; subst; done.
-Qed.
-
-(* up to seplog *)
-Lemma gvar_agree : forall i b1 b2, ⊢ gvar i b1 -∗ gvar i b2 -∗ ⌜b1 = b2⌝.
-Proof.
-  intros; iIntros "H1 H2".
-  by iDestruct (own_valid_2 with "H1 H2") as %((_ & ?%to_agree_op_inv)%lib.gmap_view.gmap_view_frag_op_valid & _).
 Qed.
 
 Lemma tc_vals_length: forall tys vs, tc_vals tys vs -> length tys = length vs.
@@ -243,6 +256,261 @@ Proof.
   by iRewrite -"H".
 Qed.
 
+(*Lemma make_args_close_precondition:
+  forall bodyparams args ge tx ve' te' (P : list val -> mpred),
+    list_norepet (map fst bodyparams) ->
+    bind_parameter_temps bodyparams args tx = Some te' ->
+    Forall (fun v : val => v <> Vundef) args ->
+    P args
+   ⊢ close_precondition (map fst bodyparams) P (ge, ve', te').
+Proof.
+intros *. intros LNR BP VUNDEF.
+iIntros "P"; iExists args; iFrame; iPureIntro; repeat (split; auto).
+clear - LNR BP VUNDEF.
+generalize dependent te'. generalize dependent tx. generalize dependent args.
+induction bodyparams; simpl; intros; destruct args; inv BP; simpl; auto.
++ destruct a; discriminate.
++ destruct a. inv LNR. inv VUNDEF. simpl. erewrite <- IHbodyparams by eauto.
+  f_equal.
+  rewrite (pass_params_ni _ _ _ _ _ H0 H2) Maps.PTree.gss //.
+Qed.*)
+
+Lemma curr_env_ge : forall ge f rho, curr_env ge f rho ⊢ curr_env ge f rho ∗
+   <affine> ⌜∀ i : ident, ge_of rho !! i = Genv.find_symbol ge i⌝ ∗
+   ⎡own(inG0 := envGS_inG) env_name (lib.gmap_view.gmap_view_auth dfrac.DfracDiscarded (to_agree <$> ge_of rho), ε)⎤.
+Proof.
+  intros; iIntros "((% & %) & #$ & $)"; auto.
+Qed.
+
+Lemma var_blocks_eq : forall {CS} (ge : genv) lv rho
+  (Hcomplete : Forall (λ it : ident * type, complete_type (@cenv_cs CS) it.2 = true) lv)
+  (Hsub : cenv_sub (@cenv_cs CS) ge)
+  (Hlookup : ∀ n i t, (lv !! n)%stdpp = Some (i, t) → ∃ b : block, eval_lvar i t rho = Vptr b Ptrofs.zero),
+  ([∗ list] idt ∈ lv, var_block Share.top idt rho) ⊣⊢
+  ∃ lb, <affine> ⌜∀ n i t b, (lv !! n)%stdpp = Some (i, t) → (lb !! n)%stdpp = Some b → eval_lvar i t rho = Vptr b Ptrofs.zero⌝ ∗
+  ([∗ list] idt;b ∈ lv;lb, memory_block Share.top (@Ctypes.sizeof ge idt.2) (Vptr b Ptrofs.zero)).
+Proof.
+  induction lv as [|(i, t) lv IH]; simpl; intros.
+  - iSplit.
+    + iIntros "_"; iExists []; simpl; auto.
+    + iIntros "(% & ?)"; destruct lb; simpl; auto.
+  - inv Hcomplete.
+    rewrite IH // /var_block.
+    monPred.unseal; iSplit.
+    + iIntros "((% & ?) & % & % & ?)".
+      edestruct (Hlookup O) as (b & Heval); first done.
+      rewrite Heval -(cenv_sub_sizeof Hsub) //.
+      iExists (b :: lb); simpl; iFrame.
+      iPureIntro; intros [|]; simpl; eauto.
+      inversion 1; inversion 1; subst; done.
+    + iIntros "(% & % & H)"; destruct lb; simpl; first iDestruct "H" as "[]".
+      rewrite (H O _ _ _ eq_refl eq_refl) /= -(cenv_sub_sizeof Hsub) //.
+      iDestruct "H" as "((%Hlt & $) & $)".
+      iPureIntro; split.
+      * rewrite !Ptrofs.unsigned_zero !Z.add_0_l in Hlt |- *.
+        split3; auto; rewrite /Ptrofs.max_unsigned; lia.
+      * intros n; apply (H (S n)).
+    + intros n; apply (Hlookup (S n)).
+Qed.
+
+Lemma stackframe_of_eq : forall {CS : compspecs} (ge : genv) f0 f rho0 k lv n
+  (Hcomplete : Forall (λ it : ident * type, complete_type cenv_cs it.2 = true) (fn_vars f))
+  (Hsub : cenv_sub cenv_cs ge),
+  list_norepet (map fst (fn_vars f)) ->
+  list_norepet (map fst (fn_params f) ++ map fst (fn_temps f)) ->
+  curr_env ge f0 rho0 k ∗ stack_retainer f n ∗ stackframe_of' ge f lv n ⊢ curr_env ge f0 rho0 k ∗ 
+  ∃ rho, <affine> ⌜ge_of rho = ge_of rho0 /\ (exists lb, length lb = length (fn_vars f) /\ ve_of rho = (list_to_map (zip (map fst (fn_vars f)) (zip lb (map snd (fn_vars f)))))) /\
+    te_of rho = list_to_map (zip (map fst (fn_params f) ++ map fst (fn_temps f)) lv)⌝ ∗
+  curr_env ge f rho n ∗ stackframe_of f rho.
+Proof.
+  intros; iIntros "(Hcurr & H)".
+  iDestruct (monPred_in_entails with "Hcurr") as "Hcurr"; first by apply curr_env_ge.
+  monPred.unseal; rewrite monPred_at_affinely; iDestruct "Hcurr" as "($ & %Hge & Hge)".
+  iDestruct (monPred_in_entails with "[H]") as "H"; first by apply stackframe_of_eq'.
+  { rewrite monPred_at_sep //. }
+  rewrite monPred_at_exist; iDestruct "H" as (lb) "H".
+  rewrite /stackframe_of1; monPred.unseal.
+  iDestruct "H" as "((%Hlv & stack) & blocks)".
+  rewrite monPred_at_big_sepL2.
+  iDestruct (big_sepL2_length with "blocks") as %Hlen.
+  iExists (ge_of rho0, _, _); iSplit.
+  { iPureIntro; simpl; split3; eauto. }
+  assert (length (map fst (fn_vars f)) = length (zip lb (map snd (fn_vars f)))) as Heq1.
+  { rewrite length_zip_with_l_eq map_length //. }
+  assert (length (map fst (fn_params f) ++ map fst (fn_temps f)) = length lv) as Heq2.
+  { rewrite !app_length !map_length Hlv //. }
+  assert (NoDup (zip (map fst (fn_params f) ++ map fst (fn_temps f)) lv).*1).
+  { rewrite -norepet_NoDup fst_zip //. by rewrite Heq2. }
+  assert (NoDup (zip (map fst (fn_vars f)) (zip lb (map snd (fn_vars f)))).*1).
+  { rewrite -norepet_NoDup fst_zip //. by rewrite Heq1. }
+  iSplitL "Hge stack".
+  - rewrite /curr_env -assert_of_eq; monPred.unseal; rewrite monPred_at_affinely.
+    iSplit; last iFrame.
+    { iPureIntro; split; auto.
+      rewrite /stack_size.
+      destruct (fn_vars f); last done.
+      destruct (fn_params f); last done.
+      destruct (fn_temps f); done. }
+    rewrite !map_size_list_to_map //.
+    rewrite !length_zip_with_l_eq // map_length // app_length !map_length.
+    rewrite Nat.add_assoc //.
+  - rewrite /stackframe_of monPred_at_big_sepL /=.
+    rewrite var_blocks_eq //.
+    + iExists lb; iFrame; iPureIntro.
+      rewrite /eval_lvar /=.
+      intros ???? Hn Hb.
+      setoid_rewrite elem_of_list_to_map_1; [|try done..].
+      2: { rewrite elem_of_zip_gen /=.
+           exists n0; rewrite list_lookup_fmap Hn; split; auto.
+           rewrite lookup_zip_with Hb /= list_lookup_fmap Hn //. }
+      rewrite /= eqb_type_refl //.
+    + rewrite /eval_lvar /=.
+      intros ??? Hn.
+      pose proof (lookup_lt_Some _ _ _ Hn) as Hlt'.
+      rewrite Hlen in Hlt'.
+      apply lookup_lt_is_Some_2 in Hlt' as (? & Hb).
+      setoid_rewrite elem_of_list_to_map_1; [|try done..].
+      2: { rewrite elem_of_zip_gen /=.
+           exists n0; rewrite list_lookup_fmap Hn; split; auto.
+           rewrite lookup_zip_with Hb /= list_lookup_fmap Hn //. }
+      eexists; rewrite /= eqb_type_refl //.
+Qed.
+
+Lemma make_tycontext_t_sound : forall tys1 tys2 id t, list_norepet (map fst tys1 ++ map fst tys2) ->
+  make_tycontext_t tys1 tys2 !! id = Some t <-> In (id, t) (tys1 ++ tys2).
+Proof.
+  intros; split; first apply make_context_t_get'.
+  induction tys1; simpl in *.
+  - induction tys2; simpl; first done.
+    intros [-> | ?].
+    + apply PTree.gss.
+    + destruct a; inv H.
+      rewrite PTree.gso; auto.
+      intros ->.
+      contradiction H3; rewrite in_map_iff; eexists (_, _); eauto.
+  - intros [-> | ?].
+    + apply PTree.gss.
+    + destruct a; inv H.
+      rewrite PTree.gso; auto.
+      intros ->.
+      contradiction H3; rewrite -map_app in_map_iff; eexists (_, _); eauto.
+Qed.
+
+Lemma stackframe_of_eq' : forall {CS : compspecs} (ge : genv) Delta f rho n
+  (Htc : guard_environ (func_tycontext' f Delta) f rho)
+  (Hcomplete : Forall (λ it : ident * type, complete_type cenv_cs it.2 = true) (fn_vars f))
+  (Hsub : cenv_sub cenv_cs ge),
+  list_norepet (map fst (fn_vars f)) ->
+  list_norepet (map fst (fn_params f) ++ map fst (fn_temps f)) ->
+  curr_env ge f rho n ∗ stackframe_of f rho ⊢
+  stack_retainer f n ∗ ∃ lv, stackframe_of' ge f lv n.
+Proof.
+  intros; trans (∃ lv lb, stackframe_of1 ge f lb lv n).
+  - rewrite /curr_env /stackframe_of /stackframe_of1 -assert_of_eq /=; monPred.unseal.
+    rewrite monPred_at_affinely; iIntros "(((% & %) & _ & stack) & H)".
+    set (lv := map (λ '(i, t), force_val (lookup i (te_of rho))) (fn_params f ++ fn_temps f)).
+    set (lb := map (λ '(i, t), match lookup i (ve_of rho) with Some (b, _) => b | _ => 1%positive end) (fn_vars f)).
+    iExists lv, lb.
+    iSplitL "stack".
+    + iSplit; first by rewrite map_length app_length.
+      assert (length (map fst (fn_vars f)) = length (zip lb (map snd (fn_vars f)))) as Heq1.
+      { rewrite length_zip_with_l_eq /lb !map_length //. }
+      assert (length (map fst (fn_params f) ++ map fst (fn_temps f)) = length lv) as Heq2.
+      { rewrite !app_length /lv !map_length app_length //. }
+      assert (NoDup (zip (map fst (fn_params f) ++ map fst (fn_temps f)) lv).*1).
+      { rewrite -norepet_NoDup fst_zip //. by rewrite Heq2. }
+      assert (NoDup (zip (map fst (fn_vars f)) (zip lb (map snd (fn_vars f)))).*1).
+      { rewrite -norepet_NoDup fst_zip //. by rewrite Heq1. }
+      iStopProof; f_equiv.
+      * rewrite !map_size_list_to_map //.
+        rewrite !length_zip_with_l_eq // /lb !map_length // app_length !map_length.
+        rewrite Nat.add_assoc //.
+      * apply map_eq; intros.
+        destruct Htc as ((_ & Htc & _) & _); specialize (Htc i).
+        setoid_rewrite make_tycontext_v_sound in Htc; last done.
+        destruct (ve_of rho !! i)%stdpp as [(?, ?)|] eqn: Hve; rewrite Hve.
+        -- edestruct Htc as (_ & Htc'); spec Htc'; first eauto.
+           symmetry; apply elem_of_list_to_map; first done.
+           apply elem_of_list_In, elem_of_list_lookup_1 in Htc' as (j & Hi).
+           apply elem_of_zip_gen; exists j; rewrite list_lookup_fmap Hi; split; first done.
+           rewrite lookup_zip_with /lb !list_lookup_fmap Hi /= Hve //.
+        -- symmetry; apply not_elem_of_list_to_map_1.
+           intros ((?, ?) & -> & (? & ((?, ?) & ? & Hin%elem_of_list_In)%elem_of_list_lookup_2%elem_of_list_fmap & ?)%elem_of_zip_gen)%elem_of_list_fmap; simpl in *; subst.
+           apply Htc in Hin as (? & ?); done.
+      * apply map_eq; intros.
+        destruct Htc as ((Htc & _) & Hf & _); specialize (Htc i); specialize (Hf i); simpl in *.
+        unfold isSome in Hf.
+        setoid_rewrite make_tycontext_t_sound in Htc; last done.
+        setoid_rewrite make_tycontext_t_sound in Hf; last done.
+        destruct (te_of rho !! i)%stdpp eqn: Hte; rewrite Hte.
+        -- destruct (Hf _ Hte) as (? & Hi).
+           symmetry; apply elem_of_list_to_map; first done.
+           apply elem_of_list_In, elem_of_list_lookup_1 in Hi as (j & Hi).
+           apply elem_of_zip_gen; exists j; rewrite -map_app list_lookup_fmap Hi; split; first done.
+           rewrite /lv list_lookup_fmap Hi /= Hte //.
+        -- symmetry; apply not_elem_of_list_to_map_1.
+           intros ((?, ?) & -> & (? & Hin%elem_of_list_lookup_2 & ?)%elem_of_zip_gen)%elem_of_list_fmap; simpl in *; subst.
+           rewrite -map_app in Hin; apply elem_of_list_fmap in Hin as ((?, ?) & -> & Hin%elem_of_list_In).
+           apply Htc in Hin as (? & ? & ?); done.
+    + rewrite monPred_at_big_sepL monPred_at_big_sepL2 var_blocks_eq //.
+      setoid_rewrite monPred_at_embed.
+      iDestruct "H" as (lb1 Hlb1) "H"; simpl.
+      iDestruct (big_sepL2_length with "H") as %Hlen.
+      assert (lb1 = lb) as ->; last done.
+      { eapply list_eq_same_length; eauto; unfold lb.
+        { rewrite map_length //. }
+        intros ?????.
+        rewrite list_lookup_fmap.
+        destruct (fn_vars f !! i)%stdpp as [(?, ?)|] eqn: Hf; inversion 1.
+        eapply Hlb1 in Hf; last done.
+        rewrite /eval_lvar in Hf.
+        destruct (ve_of rho !! i0)%stdpp as [(?, ?)|]; last done.
+        destruct (eqb_type t t0); inv Hf; done. }
+      intros ??? Hf; rewrite /eval_lvar.
+      destruct Htc as ((_ & Htc & _) & _).
+      specialize (Htc i t); simpl in Htc.
+      rewrite make_tycontext_v_sound // in Htc.
+      apply elem_of_list_lookup_2, elem_of_list_In, Htc in Hf as (? & ->).
+      rewrite eqb_type_refl; eauto.
+  - iIntros "(% & % & H)".
+    iDestruct (monPred_in_entails with "H") as "H"; first by apply stackframe_of_eq1'.
+    rewrite monPred_at_sep; iDestruct "H" as "($ & $)".
+Qed.
+
+Lemma tc_vals_Vundef {args ids} (TC:tc_vals ids args): Forall (fun v : val => v <> Vundef) args.
+Proof.
+generalize dependent ids. induction args; intros. constructor.
+destruct ids; simpl in TC. contradiction. destruct TC.
+constructor; eauto. intros N; subst. apply (tc_val_Vundef _ H).
+Qed.
+
+Lemma tc_vals_lookup {args ids} (TC:tc_vals ids args):
+  forall n i v, lookup n ids = Some i -> lookup n args = Some v -> tc_val i v.
+Proof.
+  generalize dependent ids; induction args; destruct ids; simpl; try done.
+  intros (? & ?); destruct n; simpl.
+  - inversion 1; inversion 1; by subst.
+  - eauto.
+Qed.
+
+Lemma repeat_lookup : forall {A} (x : A) m n, lookup n (repeat x m) =
+  if decide (n < m)%nat then Some x else None.
+Proof.
+  induction m; simpl.
+  - apply lookup_nil.
+  - destruct n; simpl; first done.
+    rewrite IHm; repeat if_tac; try done; lia.
+Qed.
+
+Lemma bind_ret_eq : forall vl t Q, bind_ret vl t Q ⊣⊢
+  <affine> ⌜match vl with Some v => tc_val t v | None => t = Tvoid end⌝ ∗ ⎡Q vl⎤.
+Proof.
+  intros; rewrite /bind_ret; destruct vl; simpl.
+  - iSplit; iIntros "($ & $)".
+  - destruct t; [|rewrite bi.pure_False // bi.affinely_False bi.sep_False //..].
+    rewrite bi.pure_True // bi.affinely_True_emp bi.emp_sep //.
+Qed.
+
 Lemma semax_call_si:
   forall E Delta (A: TypeTree) (Ef : dtfr (MaskTT A))
    (P : dtfr (ArgsTT A))
@@ -264,7 +532,7 @@ Proof.
   intros.
   rewrite semax_unfold; intros.
   destruct HGG.
-  iIntros "E F #B" (f0 (TC' & ?)) "Pre".
+  iIntros "F #B" (f0 ? (TC' & ?)) "E Pre".
   rewrite monPred_at_and monPred_at_sep !monPred_at_later monPred_at_and monPred_at_sep /=.
   iAssert ⎡func_ptr_si (mk_funspec (argsig, retsig) cc A Ef P Q) (eval_expr(CS := CS) a rho)⎤ as "#fp".
   { iDestruct "Pre" as "(_ & $ & _)". }
@@ -288,11 +556,12 @@ Proof.
   destruct Hid as (-> & Hid).
   iDestruct "F" as "(_ & _ & F)".
   iDestruct "sub" as "(_ & sub)".
-  iSpecialize ("B" with "[g]").
-  { iIntros "!>"; iExists id; iFrame "g"; eauto. }
+  iDestruct (curr_env_gvar_e with "[$E $g]") as %Hsymb.
+  iPoseProof ("B" with "[%]") as "B'".
+  { exists id; eauto. }
   assert (cenv_sub (@cenv_cs CS) psi) by (eapply cenv_sub_trans; eauto).
   pose proof (typecheck_environ_sub _ _ TS _ TC') as TC.
-  iDestruct "B" as "[BE|BI]".
+  iDestruct "B'" as "[BE|BI]".
   - iApply wp_extcall.
     iApply (wp_tc_expr(CS := CS) with "E"); [done..|].
     iSplit; first by rewrite !bi.and_elim_l; auto.
@@ -312,7 +581,7 @@ Proof.
     iMod (fupd_mask_subseteq (fE fx)) as "Hclose'"; first done.
     iMod ("BE" $! _ _ emp with "[Pre]") as "Hext".
     { iStopProof; split => ?; monPred.unseal.
-      rewrite monPred_at_intuitionistically /=; iIntros "(#(_ & _ & _ & HP & _) & Pre)".
+      rewrite monPred_at_intuitionistically /=; iIntros "(#(_ & _ & _ & _ & HP & _) & Pre)".
       rewrite bi.sep_emp.
       rewrite ofe_morO_equivI; iSpecialize ("HP" $! fx).
       rewrite discrete_fun_equivI; iSpecialize ("HP" $! (eval_exprlist l bl rho)).
@@ -358,7 +627,7 @@ Proof.
       * iPureIntro.
         destruct TS as (TS & _); specialize (TS i). rewrite Hi in TS.
         destruct (temp_types Delta' !! i) eqn: ?; inv TS.
-        eapply typecheck_environ_set; eauto.
+        eapply guard_environ_put_te'; eauto; first by split.
         apply tc_val_tc_val'; auto.
     + iFrame.
       iSplit; last done.
@@ -386,48 +655,120 @@ Proof.
     iSplit; first by rewrite bi.and_elim_l bi.and_elim_r; auto.
     iIntros "E" (TCargs).
     exploit tc_vals_length; first done; intros Hlen; rewrite -Hlen map_length; iSplit; first done.
-    iSpecialize ("BI" $! psi with "[//]").
+    iSpecialize ("BI" with "[%] [%]").
+    { intros; apply tycontext_sub_refl. }
+    { apply cenv_sub_refl. }
     iNext.
     iStopProof; split => n; simpl.
     rewrite !monPred_at_sep -assert_of_eq
-      monPred_at_big_sepM monPred_at_intuitionistically monPred_at_affinely !monPred_at_and
-      !monPred_at_embed monPred_at_pure !monPred_at_internal_eq monPred_at_wand.
-    iIntros "(#(sub & func & g & HP & HQ & BI) & Pre & F & E)" (? [=]) "stack".
+      monPred_at_intuitionistically monPred_at_affinely !monPred_at_and
+      !monPred_at_embed monPred_at_pure !monPred_at_internal_eq monPred_at_wand monPred_at_forall.
+    iIntros "(#(B & sub & func & g & HP & HQ & BI) & Pre & F & E)" (? [=]) "stack0".
+    rewrite monPred_at_wand.
+    iIntros (? [=]) "stack".
     rewrite monPred_at_later; iNext.
-    rewrite monPred_at_plainly.
-    iSpecialize ("BI" $! j); rewrite monPred_at_forall.
     iDestruct "Pre" as "(_ & _ & Frame & Pre)".
     rewrite -fupd_wp monPred_at_fupd.
     iMod (fupd_mask_subseteq (Ef x)) as "Hclose"; first done.
     iMod ("sub" with "[$Pre]") as (fx F0 ?) "((F0 & Pre) & #Post)".
     { iPureIntro. by split; first apply tc_vals_HaveTyps. }
     iSpecialize ("BI" $! fx).
-    rewrite monPred_at_wand.
+    rewrite semax_fold_unfold; monPred.unseal.
+    iSpecialize ("BI" with "[//] [%]").
+    { split3; eauto; [apply tycontext_sub_refl | apply cenv_sub_refl]. }
+    subst; iDestruct (stackframe_of_eq with "[E stack0 stack]") as "(E & % & %Hrho & E' & stack)"; [done..| |].
+    { iFrame.
+      rewrite /curr_env; monPred.unseal.
+      rewrite monPred_at_affinely -assert_of_eq; iFrame. }
+    iSpecialize ("BI" $! (S n) with "[//] F [//] [B] [//]").
+    { rewrite -(plain_plainly (believe _ _ _ _)) !monPred_at_plainly //. }
+    assert (NoDup (zip (map fst (fn_params f) ++ map fst (fn_temps f))
+        (eval_exprlist(CS := CS) (type_of_params (fn_params f)) bl rho ++ repeat Vundef (length (fn_temps f)))).*1).
+    { rewrite -norepet_NoDup fst_zip //.
+      rewrite map_length in Hlen; rewrite !app_length !map_length Hlen repeat_length //. }
+    assert (forall n i t, lookup n (fn_params f) = Some (i, t) ->
+        exists v, lookup n (eval_exprlist(CS := CS) (type_of_params (fn_params f)) bl rho) = Some v /\
+          lookup i (te_of rho0) = Some v) as Hte.
+    { intros ??? Hn.
+      pose proof (lookup_lt_Some _ _ _ Hn) as Hlt.
+      rewrite map_length in Hlen; rewrite Hlen in Hlt.
+      apply lookup_lt_is_Some_2 in Hlt as (? & ?).
+      eexists; split; first done.
+      destruct Hrho as (_ & _ & ->).
+      apply elem_of_list_to_map; first done.
+      apply elem_of_zip_gen.
+      exists n0; rewrite -map_app list_lookup_fmap; erewrite !lookup_app_l_Some by done; done. }
+    iSpecialize ("BI" with "[] [//] E'").
+    { destruct Hrho as (Hge0 & (lb & Hlb & Hve0) & Hte0).
+      rewrite monPred_at_affinely; iPureIntro; split3; last done.
+      split3.
+      + intros ?? Hi%make_context_t_get'.
+        apply in_app_iff in Hi as [Hi | Hi].
+        * apply elem_of_list_In, elem_of_list_lookup_1 in Hi as (? & Hi).
+          edestruct Hte as (? & ? & ->); first done.
+          eexists; split; first done.
+          eapply tc_val_tc_val', tc_vals_lookup; eauto.
+          rewrite list_lookup_fmap Hi //.
+        * apply elem_of_list_In, elem_of_list_lookup_1 in Hi as (i & Hi).
+          pose proof (lookup_lt_Some _ _ _ Hi) as Hlt.
+          exists Vundef; split; last by intros ?.
+          rewrite Hte0; apply elem_of_list_to_map; first done.
+          apply elem_of_zip_gen.
+          exists (length (fn_params f) + i)%nat.
+          rewrite !lookup_app_r; rewrite -?Hlen ?map_length; try lia.
+          rewrite !Nat.add_sub' list_lookup_fmap Hi; split; first done.
+          rewrite repeat_lookup if_true //.
+      + intros ??; rewrite make_tycontext_v_sound //.
+        assert (NoDup (zip (map fst (fn_vars f)) (zip lb (map snd (fn_vars f)))).*1).
+        { rewrite -norepet_NoDup fst_zip // length_zip_with_l_eq map_length //; lia. }
+        rewrite Hve0; split.
+        * intros Hi.
+          apply elem_of_list_In, elem_of_list_lookup_1 in Hi as (i & Hi).
+          pose proof (lookup_lt_Some _ _ _ Hi) as Hb.
+          rewrite -Hlb in Hb; apply lookup_lt_is_Some_2 in Hb as (? & Hb).
+          eexists; apply elem_of_list_to_map; first done.
+          apply elem_of_zip_gen.
+          exists i; rewrite lookup_zip_with Hb /= !list_lookup_fmap Hi //.
+        * intros (? & Hi%elem_of_list_to_map); last done.
+          apply elem_of_zip_gen in Hi as (i & Hi & Hb).
+          rewrite lookup_zip_with in Hb; apply bind_Some in Hb as (? & ? & Hb).
+          rewrite !list_lookup_fmap in Hi Hb.
+          apply bind_Some in Hb as (? & Hb & [=]); subst.
+          apply elem_of_list_In, (elem_of_list_lookup_2 _ i).
+          destruct (lookup i (fn_vars f)) as [(?, ?)|] eqn: Hl; inv Hi; inv Hb; done.
+      + rewrite Hge0; apply TC'.
+      + simpl.
+        rewrite Hte0.
+        setoid_rewrite make_tycontext_t_sound; last done.
+        intros ?? Hi%elem_of_list_to_map; last done.
+        apply elem_of_zip_gen in Hi as (? & Hi%elem_of_list_lookup_2%elem_of_list_In & _).
+        rewrite -map_app in Hi; apply in_map_iff in Hi as ((?, ?) & [=] & ?); subst; eauto. }
     iSpecialize ("BI" with "[//] [stack Pre]").
-    { rewrite /bind_args /close_precondition monPred_at_sep monPred_at_and monPred_at_exist.
-      rewrite map_length in Hlen.
-      subst; iSplit.
-      + rewrite monPred_at_absorbingly /tc_formals monPred_at_exist.
-        iExists (eval_exprlist(CS := CS) (type_of_params (fn_params f)) bl rho).
-        rewrite monPred_at_and monPred_at_pure !monPred_at_big_sepL2 big_sepL2_fmap_l.
-        iDestruct "stack" as "(_ & temps)".
-        iDestruct (big_sepL2_app_inv with "temps") as "($ & _)"; first auto.
-        iPureIntro; auto.
+    { iFrame.
+      rewrite /bind_args monPred_at_and /=; iSplit.
+      + iPureIntro.
+        rewrite /tc_formals.
+        match goal with H: tc_vals _ ?A |- tc_vals _ ?B => replace B with A; auto end.
+        eapply list_eq_same_length; eauto.
+        { rewrite -Hlen !map_length //. }
+        intros ?????.
+        rewrite list_lookup_fmap; destruct (lookup i (fn_params f)) as [(?, ?)|] eqn: Hi; inversion 1; subst.
+        rewrite /eval_id.
+        apply Hte in Hi as (? & ? & ->); simpl; congruence.
       + rewrite ofe_morO_equivI; iSpecialize ("HP" $! fx).
         rewrite discrete_fun_equivI; iSpecialize ("HP" $! (eval_exprlist (map snd (fn_params f)) bl rho)).
-        iExists _; rewrite monPred_at_and !monPred_at_sep monPred_at_embed monPred_at_pure /type_of_params; subst; iFrame.
-        iSplit.
-        { iPureIntro.
-          clear - TCargs.
-          fold (type_of_params (fn_params f)).
-          forget (type_of_params (fn_params f)) as tys.
-          forget (eval_exprlist tys bl rho) as vals.
-          generalize dependent tys; induction vals; destruct tys; try done; simpl.
-          intros (? & ?); constructor; eauto.
-          intros ->; by apply tc_val_Vundef in H. }
-        Fail iRewrite "HP".
-        iApply (internal_eq_app with "[] Pre").
-        by iApply (internal_eq_sym with "HP"). }
+        Fail iRewrite -"HP" in "Pre".
+        iPoseProof (internal_eq_app with "[HP] Pre") as "Pre".
+        { by iApply (internal_eq_sym with "HP"). }
+        iFrame; iPureIntro.
+        split; last done; split.
+        * rewrite map_map; eapply list_eq_same_length; eauto.
+          { rewrite !map_length -Hlen map_length //. }
+          intros ????.
+          rewrite !list_lookup_fmap; destruct (lookup i (fn_params f)) as [(?, ?)|] eqn: Hi; inversion 1; subst.
+          apply Hte in Hi as (? & He & ->).
+          rewrite He; inversion 1; done.
+        * by eapply tc_vals_Vundef. }
     iMod "Hclose" as "_"; iModIntro.
     subst.
     iApply (monPred_in_entails with "[-]"); first apply wp_mask_mono.
@@ -436,33 +777,35 @@ Proof.
     rewrite monPred_at_sep; iFrame "BI".
     iClear "HP sub"; rewrite /= /Clight_seplog.bind_ret; monPred.unseal.
     iSplit.
-    + iIntros (? [=]) "((%Hvoid & Q) & stack)".
+    + iIntros (? [=]) "((%rho' & (Q & stack) & Htc & E') & F)".
+      rewrite monPred_at_affinely; iDestruct "Htc" as %Htc.
+      destruct (fn_return f) eqn: Hret; [|done..].
+      simpl.
       rewrite ofe_morO_equivI; iSpecialize ("HQ" $! fx).
       rewrite discrete_fun_equivI; iSpecialize ("HQ" $! None).
       iRewrite "HQ" in "Q".
       iPoseProof ("Post" with "[$F0 $Q]") as "Q".
-      iIntros "!>"; iFrame "stack".
+      iIntros "!>".
+      iDestruct (stackframe_of_eq' with "[$E' $stack]") as "$"; [done..|].
       iSplit; first done.
-      specialize (TC5 Hvoid); subst; simpl.
+      specialize (TC5 eq_refl); subst; simpl.
       iFrame.
-      iSplitL "Q".
-      * iExists Vundef; by rewrite Hvoid.
-      * rewrite monPred_at_affinely /=; iSplit; first done.
-        rewrite /curr_env /= !monPred_at_sep monPred_at_affinely monPred_at_big_sepM monPred_at_pure -assert_of_eq /=.
-        setoid_rewrite monPred_at_embed; done.
-    + do 2 (iSplit; first iIntros (??) "([] & ?)").
-      iIntros (r ? [=]) "((%Hr & Q) & stack)".
+      iSplit; first by iExists Vundef.
+      rewrite monPred_at_affinely //.
+    + do 2 (iSplit; first iIntros (??) "((% & ([] & ?) & ?) & ?)").
+      iIntros (r ? [=]) "((%rho' & (Q & stack) & Htc & E') & F)".
+      rewrite monPred_at_affinely; iDestruct "Htc" as %Htc.
+      rewrite bind_ret_eq; monPred.unseal; rewrite monPred_at_affinely. iDestruct "Q" as (Hr) "Q".
       rewrite ofe_morO_equivI; iSpecialize ("HQ" $! fx).
       rewrite discrete_fun_equivI; iSpecialize ("HQ" $! r).
       iRewrite "HQ" in "Q".
       iPoseProof ("Post" with "[$F0 $Q]") as "Q".
-      iIntros "!>"; iFrame "stack".
-      iSplit; first done.
+      iDestruct (stackframe_of_eq' with "[$E' $stack]") as "$"; [done..|].
+      iIntros "!>"; iSplit; first done.
       destruct ret; subst; simpl.
       * simpl in TC7.
         destruct (temp_types Delta !! i) eqn: Hi; last done.
-        iDestruct (monPred_in_entails with "[E]") as "E"; first by eapply curr_env_set_temp.
-        { rewrite /curr_env !monPred_at_sep monPred_at_big_sepM monPred_at_affinely -assert_of_eq; monPred.unseal; done. }
+        iDestruct (monPred_in_entails with "E") as "E"; first by eapply curr_env_set_temp.
         rewrite monPred_at_sep monPred_at_exist monPred_at_forall; iDestruct "E" as "($ & E)".
         iIntros (??) "Hi".
         iSpecialize ("E" $! (force_val r)); rewrite monPred_at_wand; iSpecialize ("E" with "[//] Hi"); iFrame.
@@ -475,16 +818,14 @@ Proof.
         ++ iPureIntro.
            destruct TS as (TS & _); specialize (TS i). rewrite Hi in TS.
            destruct (temp_types Delta' !! i) eqn: ?; inv TS.
-           eapply typecheck_environ_set; eauto.
+           eapply guard_environ_put_te'; eauto; first by split.
            apply tc_val_tc_val'; auto.
       * iFrame.
         iSplitL "Q".
         ++ iExists Vundef; destruct r.
            ** destruct (fn_return f); try done; iFrame; iPureIntro; by split; first apply tc_val_tc_val'.
            ** by rewrite Hr.
-        ++ rewrite monPred_at_affinely /=; iSplit; first done.
-           rewrite /curr_env /= !monPred_at_sep monPred_at_affinely monPred_at_big_sepM monPred_at_pure -assert_of_eq /=.
-           setoid_rewrite monPred_at_embed; done.
+        ++ rewrite monPred_at_affinely //.
 Qed.
 
 (* We need the explicit frame because it might contain typechecking information. *)
@@ -567,7 +908,7 @@ Proof.
   destruct HGG as [CSUB HGG].
   replace (ret_type Delta) with (ret_type Delta')
     by (destruct TS as [_ [_ [? _]]]; auto).
-  iIntros "E F #?" (? (TC' & Hret)) "H".
+  iIntros "F #?" (?? (TC' & ? & Hret)) "E H".
   iApply wp_return.
   rewrite -Hret.
   assert (cenv_sub (@cenv_cs CS) psi) by (eapply cenv_sub_trans; eauto).
