veric/semax_straight.v
@@ -66,7 +66,7 @@ forall E (Delta: tycontext) (P: assert) id cmp e1 e2 ty sh1 sh2,
 Proof.
   intros until sh2. intros ?? CMP NE1 NE2 TCid.
   rewrite semax_unfold; intros. destruct HGG.
-  iIntros "E F #?" (? (TC' & ?)) "Pre".
+  iIntros "F #?" (?? (TC' & ?)) "E Pre".
   rewrite monPred_at_later !monPred_at_and.
   iApply wp_set. iApply wp_binop_rule.
   assert (cenv_sub (@cenv_cs CS) psi) by (eapply cenv_sub_trans; eauto).
@@ -104,7 +104,7 @@ Proof.
   - iPureIntro.
     destruct TS as (TS & _); specialize (TS id). rewrite Hi in TS.
     destruct (temp_types Delta' !! id) eqn: ?; inv TS.
-    eapply typecheck_environ_set; eauto.
+    eapply guard_environ_put_te'; eauto; first by split.
     apply tc_val'_sem_cmp; auto.
 Qed.
 
@@ -120,7 +120,7 @@ forall E (Delta: tycontext) (P: assert) id e,
 Proof.
   intros.
   rewrite semax_unfold; intros. destruct HGG.
-  iIntros "E ? #?" (? (TC' & ?)) "Pre".
+  iIntros "? #?" (?? (TC' & ?)) "E Pre".
   rewrite monPred_at_later !monPred_at_and.
   iApply wp_set.
   assert (cenv_sub (@cenv_cs CS) psi) by (eapply cenv_sub_trans; eauto).
@@ -146,7 +146,7 @@ Proof.
     iPureIntro.
     destruct TS as (TS & _); specialize (TS id). rewrite Ht in TS.
     destruct (temp_types Delta' !! id) eqn: ?; inv TS.
-    eapply typecheck_environ_set; eauto.
+    eapply guard_environ_put_te'; eauto; first by split.
     by apply tc_val_tc_val'.
 Qed.
 
@@ -190,7 +190,7 @@ forall E (Delta: tycontext) (P: assert) id e t
 Proof.
   intros.
   rewrite semax_unfold; intros. destruct HGG.
-  iIntros "E ? #?" (? (TC' & ?)) "Pre".
+  iIntros "? #?" (?? (TC' & ?)) "E Pre".
   rewrite monPred_at_later !monPred_at_and.
   iApply wp_set.
   assert (cenv_sub (@cenv_cs CS) psi) by (eapply cenv_sub_trans; eauto).
@@ -213,7 +213,7 @@ Proof.
     iPureIntro.
     destruct TS as (TS & _); specialize (TS id). rewrite Ht in TS.
     destruct (temp_types Delta' !! id) eqn: ?; inv TS.
-    eapply typecheck_environ_set; eauto.
+    eapply guard_environ_put_te'; eauto; first by split.
     by apply tc_val_tc_val'.
     { by apply typecheck_expr_sound. }
 Qed.
@@ -248,7 +248,7 @@ forall E (Delta: tycontext) sh id (P: assert) e1 t2 (v2: val),
 Proof.
   intros until v2.
   intros Hid0 TC1 H_READABLE H99.
-  rewrite semax_unfold; intros; iIntros "E F #?" (? (TC' & ?)) "Pre"; destruct HGG.
+  rewrite semax_unfold; intros; iIntros "F #?" (?? (TC' & ?)) "E Pre"; destruct HGG.
   rewrite monPred_at_later !monPred_at_and monPred_at_pure.
   iApply wp_set.
   assert (cenv_sub (@cenv_cs CS) psi) by (eapply cenv_sub_trans; eauto).
@@ -278,7 +278,7 @@ Proof.
   - iPureIntro.
     destruct TS as (TS & _); specialize (TS id). rewrite Ht in TS.
     destruct (temp_types Delta' !! id) eqn: ?; inv TS.
-    eapply typecheck_environ_set; eauto.
+    eapply guard_environ_put_te'; eauto; first by split.
     eapply tc_val_tc_val', neutral_cast_subsumption; eauto.
 Qed.
 
@@ -318,7 +318,7 @@ forall E (Delta: tycontext) sh id (P: assert) e1 t1 (v2: val),
 Proof.
   intros until v2.
   intros Hid0 HCAST H_READABLE H99.
-  rewrite semax_unfold; intros; iIntros "E F #?" (? (TC' & ?)) "Pre"; destruct HGG.
+  rewrite semax_unfold; intros; iIntros "F #?" (?? (TC' & ?)) "E Pre"; destruct HGG.
   rewrite monPred_at_later !monPred_at_and.
   iApply wp_set; iApply wp_cast; first done.
   iApply wp_expr_mono; first by intros; iIntros "H"; iApply "H".
@@ -360,7 +360,7 @@ Proof.
   - iPureIntro.
     destruct TS as (TS & _); specialize (TS id). rewrite Ht in TS.
     destruct (temp_types Delta' !! id) eqn: ?; inv TS.
-    eapply typecheck_environ_set; eauto.
+    eapply guard_environ_put_te'; eauto; first by split.
     by apply tc_val_tc_val'.
 Qed.
 
@@ -411,7 +411,7 @@ Lemma semax_store:
           (normal_ret_assert (assert_of (`(mapsto sh (typeof e1)) (eval_lvalue e1) (`force_val (`(sem_cast (typeof e2) (typeof e1)) (eval_expr e2)))) ∗ P)).
 Proof.
   intros.
-  rewrite semax_unfold; intros; iIntros "E ? #?" (? (TC' & ?)) "Pre"; destruct HGG.
+  rewrite semax_unfold; intros; iIntros "? #?" (?? (TC' & ?)) "E Pre"; destruct HGG.
   rewrite monPred_at_later !monPred_at_and.
   iApply wp_store.
   assert (cenv_sub (@cenv_cs CS) psi) by (eapply cenv_sub_trans; eauto).
@@ -455,7 +455,7 @@ Lemma semax_store_union_hack:
 Proof.
   intros until P. intros NT AM0 AM' OK WS.
   assert (SZ := decode_encode_val_size _ _ OK).
-  rewrite semax_unfold; intros; iIntros "E ? #?" (? (TC' & ?)) "Pre"; destruct HGG.
+  rewrite semax_unfold; intros; iIntros "? #?" (?? (TC' & ?)) "E Pre"; destruct HGG.
   rewrite monPred_at_later !monPred_at_and.
   iApply wp_store'; [done..|].
   assert (cenv_sub (@cenv_cs CS) psi) by (eapply cenv_sub_trans; eauto).
